---
layout: post
title: "Math Foundations 010 - Arithmetic with Fractions"
description: Prof Norman J Wildberger's Math Foundations (A) Lecture 10
category: math
tags: [wildberger]
comments: true
---

<head><script async='async' src='https://cdnjs.cloudflare.com/ajax/libs/mathjax/2.7.1/MathJax.js?config=TeX-AMS_CHTML,Safe' type='text/javascript'></script></head>
To review:

<p>Num or Natural Numbers: I, II, III, ...</p>

<p>Fra or Fractions: m/n where m, n, \(\in\) Num</p>

<p>\(\in\) this symbol means "are" or "is" according to wildberger. But I believe that to be specific, the symbol means "is an element of"</p>

<p>Fractions also have a notion of equality, and this happens when</p>

<p>m/n =  k\(\ell\) \(\Leftrightarrow\) m\(\ell\) = nk</p>

<p>With the given notion of equality, we are left with a question:</p>
<!-- more --> 

<center><p><u>Does m/n =  k\(\ell\)  and k\(\ell\) = p/q imply m/n = p/q?</u></p></center>

<p>The answer is yes.</p>
<p>The first statement: m/n =  k\(\ell\)</p>
<p>m\(\ell\) = nk</p>
<p>The second statement: k\(\ell\) = p/q</p>
<p>kq = \(\ell\)p</p>
<p>Then</p>
<p>(m\(\ell\))(kq) = (nk)(\(\ell\)p)</p>
<p>So</p>
<p>(mq)(\(\ell\)k) = (np)(\(\ell\)k)</p>
<p>Thus</p>
<p>mq = np</p>

<center><p>Basic fact</p></center>

<p>ab = ac \(\Rightarrow\) b = c</p>
<p>The above notation is read as: if ab is equal (=) to ac, then we deduce (\(\Rightarrow\))that b is equal to c</p>
<p>Explained: if a multiple of a is equal to another multiple of a, then those two would have to be the same</p>

<center><p>Sum of two fractions</p></center>

<p>\(\frac{a}{b}\) + \(\frac{c}{d}\) = \(\frac{ad}{bd}\) + \(\frac{bc}{bd}\)</p>
<p>= \(\frac{ad + bc}{bd}\)</p>
<p>To explain what happened here</p>

<ul>
 <li><p><big>Recall the laws of division for natural numbers (link)</big></p></li>
 <li><p><big>Recall as well that we use the horizontal line for division, and slanted line for fraction</big></p></li>
 <li><p><big>\(\frac{a}{b}\) + \(\frac{c}{d}\) </big></p></li>
  <ul>
    <li><p><big>we read this as: a divided by b plus c divided by d</big></p></li>
  </ul>
  <li><p><big>this can be rewritten to \(\frac{ad}{bd}\) + \(\frac{bc}{bd}\)</big></p></li>
  <ul>
    <li><p><big>we rewrite \(\frac{a}{b}\) to \(\frac{ad}{bd}\)</big></p></li>
    <li><p><big>we rewrite \(\frac{c}{d}\) to \(\frac{bc}{bd}\)</big></p></li>
    <li><p><big>we do this to make the denominators equal</big></p></li>
    <li><p><big>if the denominators are equal, we can add the two divisions by adding the numerator, we end up with </big></p></li>
    <ul>
      <li><p><big>= \(\frac{ad + bc}{bd}\)</big></p></li>
    </ul>
  </ul>
 <li><p><big>Referring the expression \(\frac{ad + bc}{bd}\), we then define addition operation for fractions of natural numbers as:</big></p></li>
  <ul>
    <li><p><big>a/b + c/d = (ad + bc) / (bd)</big></p></li>
    <li><p><big>For example: 2/3 + 5/4</big></p></li>
    <ul>
      <li><p><big>2/3 + 5/4 = (2 \(\times\) 4 + 3 \(\times\) 5) / (3 \(\times\) 4)</big></p></li>
      <li><p><big>= 23/12</big></p></li>
      <li><p><big>or</big></p></li>
      <ul>
        <li><p><big>\(\frac{a}{b}\) + \(\frac{c}{d}\) =  \(\frac{ad +bc}{bd}\)</big></p></li>
        <li><p><big>\(\frac{2}{3}\) +  \(\frac{5}{4}\) =  \(\frac{2 \times\ 4 + 3 \times\ 5}{3 \times\ 4}\)</big></p></li>
        <li><p><big>\(\frac{23}{12}\)</big></p></li>
      </ul>
    </ul>
  </ul>
</ul>
