---
layout: post
title: "Math Foundations 002 - Arithmetics with Numbers"
description: Prof Norman J Wildberger's Math Foundations (A) Lecture 2
category: math
tags: [wildberger]
comments: true
---



<p><span style="background-color: white; color: #222222; ">To review from the previous math foundations post, a natural number is a string of |s or 1s.</span></p><p>In this blog post, we discuss the most important laws in mathematics.

<!-- more --> 

</p><p>Laws for Addition</p><p>The&nbsp;<span style="box-sizing: inherit; ">sum</span>&nbsp;of numbers n and m is the combination of the strings of |s or 1s and is written as&nbsp;<span style="box-sizing: inherit; ">n + m</span>. By combination, we mean put together, not something like say permutation. In computer science, we illustrate this by concatenation.</p><p>Commutative Law<p>We can change the order of elements between two numbers, and we’d still arrive with the same sum</p><p>n + m = m + n</p><p>We can illustrate this by<p>| | | | | | + | | = | | | | | | | |</p><p>of which the above is equal to:</p><p>| | + | | | | | | = | | | | | | | |</p></p></p><p>Associative Law<p>As we’ve already agreed that addition is the operation of combining two numbers, we’d more than 2 numbers, we can combine two numbers first, and then add that result to the other. We can group the order of elements any way we want and we’d still arrive with the same sum.</p><p>(k + n) + m = k + (n + m)</p><p>Let’s illustrate this (we underline the result of the grouping for this illustration)<p>(k + n) + m<p>(| | + | | |) + | | | |</p><p><span style="box-sizing: inherit; text-decoration-line: underline;">| | | | |</span>&nbsp;+ | | | |</p><p><span style="box-sizing: inherit; text-decoration-line: underline;">| | | | | | | | |</span></p></p><p>k + (n + m)<p>| | + ( | | | + | | | |)</p><p>| | +&nbsp;<span style="box-sizing: inherit; text-decoration-line: underline;">| | | | | | |</span></p><p><span style="box-sizing: inherit; text-decoration-line: underline;">| | | | | | | | |</span></p></p><p>Whatever order we concatenate them, it arrives with the same string</p></p></p><p>Successor operation can be written as<p>n + 1 = s(n)</p></p><p>Laws for Multiplication</p><p>The product of numbers&nbsp;<span style="box-sizing: inherit; ">n</span>&nbsp;and&nbsp;<span style="box-sizing: inherit; ">m</span>&nbsp;is the string formed by a copy of m for every | in&nbsp;<span style="box-sizing: inherit; ">n</span>. It is written as&nbsp;<span style="box-sizing: inherit; ">n x m</span></p><p>Let’s illustrate mulitplication before we talk about laws. There are 3 elements, each with equal amount of strokes. We’d like to know how many strokes there are together:</p><p>| | | |</p><p>| | | |</p><p>| | | |</p><p>This is a matter of combining | | | | + | | | | + | | | | or we can rewrite it as 3 times 4 or | | | x | | | | which means 3 groups of four. Or we can think of it as replacing each | in the first string (| | |) with a copy of the second string (| | | |):</p><p><span class="has-inline-color has-vivid-purple-color" style="box-sizing: inherit; color: #9b51e0;">|</span>&nbsp;<span class="has-inline-color has-vivid-green-cyan-color" style="box-sizing: inherit; color: #00d084;">|</span>&nbsp;<span class="has-inline-color has-luminous-vivid-orange-color" style="box-sizing: inherit; color: #ff6900;">|</span>&nbsp;x | | | |</p><p><span class="has-inline-color has-vivid-purple-color" style="box-sizing: inherit; color: #9b51e0;">| | | |</span>&nbsp;<span class="has-inline-color has-vivid-green-cyan-color" style="box-sizing: inherit; color: #00d084;">| | | |</span>&nbsp;<span class="has-inline-color has-luminous-vivid-orange-color" style="box-sizing: inherit; color: #ff6900;">| | | |</span></p><p>Now, let’s list the laws of multiplication.</p><p>Commutative Law<p><span style="box-sizing: inherit; ">n x m = m x n</span></p><p>Like addition, we can rearrange the elements, and we’d still get the same result for the multiplication operation. Let us illustrate.<p>Suppose n is | | and m is | | |</p><p><span class="has-inline-color has-vivid-green-cyan-color" style="box-sizing: inherit; color: #00d084;">|</span>&nbsp;<span class="has-inline-color has-luminous-vivid-orange-color" style="box-sizing: inherit; color: #ff6900;">|</span>&nbsp;x | | | =&nbsp;<span class="has-inline-color has-vivid-green-cyan-color" style="box-sizing: inherit; color: #00d084;">| | |&nbsp;</span><span class="has-inline-color has-vivid-red-color" style="box-sizing: inherit; color: #cf2e2e;">| | |</span></p><p>Rearranging it, it would be&nbsp;<span class="has-inline-color has-pale-pink-color" style="box-sizing: inherit; color: #f78da7;">|</span>&nbsp;<span class="has-inline-color has-luminous-vivid-amber-color" style="box-sizing: inherit; color: #fcb900;">|</span>&nbsp;<span class="has-inline-color has-vivid-green-cyan-color" style="box-sizing: inherit; color: #00d084;">|</span>&nbsp;x | | =&nbsp;<span class="has-inline-color has-pale-pink-color" style="box-sizing: inherit; color: #f78da7;">| |</span>&nbsp;<span class="has-inline-color has-luminous-vivid-amber-color" style="box-sizing: inherit; color: #fcb900;">| |</span>&nbsp;<span class="has-inline-color has-vivid-green-cyan-color" style="box-sizing: inherit; color: #00d084;">| |</span></p></p></p><p>Identity Law<p><span style="box-sizing: inherit; ">n x 1 = n</span></p><p>Anything multiplied to 1, the product is still itself. The reasoning is that we are creating n groups of 1, and thus with the way we discuss multiplication with |s, 3 groups of | would be:<p><span class="has-inline-color has-vivid-purple-color" style="box-sizing: inherit; color: #9b51e0;">|</span>&nbsp;<span class="has-inline-color has-vivid-green-cyan-color" style="box-sizing: inherit; color: #00d084;">|</span>&nbsp;<span class="has-inline-color has-luminous-vivid-orange-color" style="box-sizing: inherit; color: #ff6900;">|</span>&nbsp;x | = | | |</p></p></p><p>Associative Law<p><span style="box-sizing: inherit; ">(k x n) x m = k x (n x m)</span></p><p>Operations in the parenthesis are done first.</p><p>Suppose k is |</p><p>Suppose n is | |</p><p>and suppose m is | | |</p><p>The left side or&nbsp;<span style="box-sizing: inherit; ">(k x n) x m</span>&nbsp;: we evaluate&nbsp;<span style="box-sizing: inherit; ">k x n</span>&nbsp;first, where we do the identity law as | x | |. Then multiply the resulting | | to m which is | | |. This results to | | | | | |, which is 2 groups of 6, our final product.</p><p>The right side or&nbsp;<span style="box-sizing: inherit; ">k x (n x m)</span>&nbsp;: we perform n x m first, where the result is | | | | | | as we ask the total of strokes in 2 groups of 3 as n is | |and m is | | |. Then, we perform multiplication on the resulting | | | | | | to 1. Where we perform identity law, leaving the final product to | | | | | | or 6 strokes.</p></p><p></p><p>Distributive Laws</p><p>Now we introduce a law that combines addition and multiplication, distribute law</p><p><span style="box-sizing: inherit; ">k</span>&nbsp;x (<span style="box-sizing: inherit; ">n</span>&nbsp;+&nbsp;<span style="box-sizing: inherit; ">m</span>) = (<span style="box-sizing: inherit; ">k&nbsp;</span>x<span style="box-sizing: inherit; ">&nbsp;n</span>) + (<span style="box-sizing: inherit; ">k</span>&nbsp;x<span style="box-sizing: inherit; ">&nbsp;m</span>) or&nbsp;<span style="box-sizing: inherit; ">k&nbsp;</span>x&nbsp;<span style="box-sizing: inherit; ">n</span>&nbsp;+&nbsp;<span style="box-sizing: inherit; ">k&nbsp;</span>x&nbsp;<span style="box-sizing: inherit; ">m</span><p>Here we see that multiplication takes precedence over addition. We have to do multiplication first.</p></p><p>(<span style="box-sizing: inherit; ">k</span>&nbsp;+&nbsp;<span style="box-sizing: inherit; ">n</span>) x&nbsp;<span style="box-sizing: inherit; ">m</span>&nbsp;=&nbsp;<span style="box-sizing: inherit; ">k&nbsp;</span>x<span style="box-sizing: inherit; ">&nbsp;m</span>&nbsp;+&nbsp;<span style="box-sizing: inherit; ">n</span>&nbsp;x&nbsp;<span style="box-sizing: inherit; ">m</span></p>
